---
title: Chapter3-02. The Neyman-Peason Fundamental Lemma
book_title: Testing Statistical Hypotheses
book_chapter: 3
book_section: 2
---

## 3.2 The Neyman-Pearson Fundamental Lemma
Family of distributions is called simple if the family consists of a single element.
Otherwise, we call it composit.

Suppose $H, K$ are both simple and $X$ is discrete.
Let $$P_{0}, P_{1}$$ be corresponding distribution.
Let $S$ be criticial reagion.
Since $$P(X \in S) = \sum_{x \in S}P(X = x)$$, the problem can be stated as following optimization problem;

$$
\begin{align}
    \min
    & & &
        \sum_{x \notin S}
            P_{1}(X = x)
    \nonumber
    \\
    \mathrm{subject\ to}
    & & &
        \sum_{x \in S}
            P_{0}(X = x)
        \le
        \alpha,
        \label{chap03_3_6}
\end{align}
$$

$$
    r(x)
    :=
    \frac{
        P_{0}(X = x)
    }{
        P_{1}(X = x)
    }
$$

$$
    P_{0}(X \in S)
    =
    \sum_{x:r(x) > c}
        P(X = x)
    = \alpha
$$

### Theorem 3.2.1
* $P_{0}, P_{1}$
    * distribution of $X$
* $\mu$
    * measure over $$(\mathcal{X}, \mathcal{A})$$
* $p_{0}, p_{1}$
    * radon nikodym derivative of $P_{i}$ with respect to $\mu$
* $$H = \{P_{0}\}$$,
    * hypothesis
* $$K = \{P_{1}\}$$,
    * alternatives
* $\alpha \in [0, 1]$,

(1)

$$
\begin{eqnarray}
    \exists \phi: \text{ test},
    \
    \exists k, \gamma \in \mathbb{R}
    \
    \text{ s.t. }
    \
    \
    \mathrm{E}_{0}
    \left[
        \phi
    \right]
    & = &
        \alpha
    \label{chap03_03_07}
    \\
    \phi(x)
    & = &
            \begin{cases}
                1
                &
                    (p_{1}(x) > kp_{0}(x))
                \\
                \gamma
                &
                    (p_{1}(x) = kp_{0}(x))
                \\
                0
                &
                    p_{1}(x) < kp_{0}(x)
            \end{cases}
    \nonumber
    \\
    & = &
        1_{\{p_{1} > kp_{0}\}}(x)
        +
        \gamma
        1_{\{p_{1} = kp_{0}\}}(x)
        \quad
        \mu
        \text{-a.e. } x
    \label{chap03_03_08}
\end{eqnarray}
$$

(2) If test $\phi$ satisifes $$\eqref{chap03_03_07}$$ and $$\eqref{chap03_03_08}$$, then $\phi$ is most powerful test at level $\alpha$.

(3) If $\alpha \in (0, 1)$ and test $\phi$ is the most powerful test at level $\alpha$, then there exists $k, \gamma \in \mathbb{R}$ such that $$\eqref{chap03_03_08}$$ satisfies.

### proof.
**proof of (1)**

For $\alpha = 0$,

$$
\begin{eqnarray}
    F(z)
    & := &
        P_{0}
        \left(
            \left\{
                x \in \mathcal{X}
                \mid
                p_{1}(x) \le z p_{0}(x)
            \right\}
        \right)
    \nonumber
    \\
    & = &
        \int_{\mathcal{X}}
            1_{\{\frac{p_{1}}{p_{0}} \le z\}}(x)
            p_{0}(x)
        \ \mu(dx)
    \label{theorem_fundamental_neyman_peason_lemma_02_def_of_cdf}
\end{eqnarray}
$$

$F$ is cumulative distribution function, that is, $F$ satisfies following propeties:

* (a) $F(+\infty) = 1$,
* (b) $F(-\infty) = 0$,
* (c) $F$ is right continuous,
* (d) $F$ is non decreasing.

Indeed, for (a), by monoton convergence theorem, we have

$$
\begin{eqnarray}
    \int_{\mathcal{X}}
        1_{\{x \mid \frac{p_{1}(x)}{p_{0}(x)} \le z\}}(x)
        p_{0}(x)
    \ \mu(dx)
    & \nearrow  &
        \int_{\mathcal{X}}
            p_{0}(x)
        \ \mu(dx)
        \quad
        (z \rightarrow \infty)
    \nonumber
    \\
    & = &
        1
    .
    \nonumber
\end{eqnarray}
$$

(b) is obivous since

$$
    P(p_{i}(x) < 0)
    =
    0
    .
$$

For (c), let $z \in \mathbb{R}$ be fixed.
For all sequence $$\{z_{n}\}_{n \in \mathbb{N}}$$, $$z_{n} \searrow z$$, we have

$$
\begin{eqnarray}
    \int_{\mathcal{X}}
        1_{\{\frac{p_{1}}{p_{0}} \le z_{n}\}}(x)
        p_{0}(x)
    \ \mu(dx)
    -
    \int_{\mathcal{X}}
        1_{\{\frac{p_{1}}{p_{0}} \le z\}}(x)
        p_{0}(x)
    \ \mu(dx)
    & = &
        \int_{\mathcal{X}}
            (
                1_{\{\frac{p_{1}}{p_{0}} \le z_{n}\}}(x)
                -
                1_{\{\frac{p_{1}}{p_{0}} \le z\}}(x)
            )
            p_{0}(x)
        \ \mu(dx)
    .
    \nonumber
\end{eqnarray}
$$

By taking the limit of equation above as $n \rightarrow \infty$, it converges to 0 by Lebesgue dominated convergence theorem.
Hence (c) holds.
Finally we show (d).
But this is obvious since integrand satisifies that

$$
    \forall z < z^{\prime},
    \
    \Rightarrow
    \
    \forall x \in \mathcal{X},
    \
    0
    \le
    1_{\{\frac{p_{1}}{p_{0}} \le z\}}(x)
    p_{0}(x)
    <
    1_{\{\frac{p_{1}}{p_{0}} \le z^{\prime}\}}(x)
    p_{0}(x)
    .
$$

Therefore, $F$ is cumulative distribution.
Since $F$ is non decreasing and right continuous,

$$
\begin{equation}
    0 < \forall \alpha < 1,
    \
    \exists k \in \mathbb{R},
    \
    \text{ s.t. }
    \
    F(k-)
    \le
    1 - \alpha
    \le
    F(k)
    .
    \label{theorem_fundamental_neyman_peason_lemma_01}
\end{equation}
$$

Indeed, let $\alpha \in (0, 1)$ be fixed.
We denote

$$
\begin{eqnarray}
    A
    & := &
        \{
            x \in \mathbb{R}
            \mid
            1 - \alpha
            \le
            F(x)
        \}
    \nonumber
    \\
    k
    & := &
        \inf
        A
    \nonumber
    \\
    B
    & := &
        \{
            x \in \mathbb{R}
            \mid
            F(x)
            \le
            1 - \alpha
        \}
    .
    \nonumber
    \\
    c
    & := &
        \sup
        B
    .
    \nonumber
\end{eqnarray}
$$

By right-continuity,

$$
    \forall \{k_{n}\},
    \
    k_{n} \searrow k,
    \
    \lim_{n \rightarrow \infty}
    F(k_{n})
    =
    F(k)
    \ge
    1 - \alpha
    .
$$

Then $F$ is non decreasing so that

$$
    \forall \{k_{n}\}_{n \in \mathbb{N}},
    \
    k_{n}
    \nearrow
    k,
    \
    \Rightarrow
    \
    k_{n}
    \le
    c
    .
$$

We can easily check this.
Suppose there exists $n$ such that $$c < k_{n}$$.
$F$ is non decreasing so that $$F(c) < F(k_{n})$$.
If $$1 - \alpha \le F(k_{n})$$, $$k_{n} \in A$$ but this contradict to $$k_{n} \le k$$.
In other hand, if we assume $$F(k_{n}) < 1 - \alpha$$, $$k_{n} \in B$$ so that $$k_{n} \le c$$.
Therefore the above statement hold.
By combining our observations, we have

$$
    \lim_{n \rightarrow \infty} F(k_{n})
    \le
    F(c)
    \le
    1 - \alpha
    \le
    F(k)
    .
$$

The equation $$\eqref{theorem_fundamental_neyman_peason_lemma_01}$$ holds.
Now we define constant $\gamma$

$$
    \gamma
    :=
    \begin{cases}
        0
        &
            F(k) = F(k-) = 1 - \alpha
        \\
        \frac{F(k) - (1 - \alpha)}{F(k) - F(k-)}
        &
            \text{otherwise}
    \end{cases}
    ,
$$

and test $\phi$

$$
    \phi(x)
    :=
    1_{\{p_{1} > k p_{0}\}}(x)
    +
    \gamma
    1_{\{p_{1} = k p_{0}\}}(x)
    .
$$

Then we have

$$
\begin{eqnarray}
    \mathrm{E}_{0}
    \left[
        \phi
    \right]
    & = &
        P_{0}(p_{1} > k p_{0})
        +
        \gamma
        P_{0}(p_{1} = k p_{0})
    \nonumber
    \\
    & = &
        1 - F(k)
        +
        \gamma
        (F(k) - F(k-))
    \nonumber
    \\
    & = &
        \begin{cases}
            1 - (1- \alpha)
            &
                F(k) = F(k-) =  1 - \alpha
            \\
            1 - F(k)
            -
            (
                F(k)
                -
                (1 - \alpha)
            )
            &
                \text{otherwise}
        \end{cases}
    \nonumber
    \\
    & = &
        \alpha
\end{eqnarray}
$$

**proof of (2)**

Let $\phi$ be test.
There exist $k, \gamma \in \mathbb{R}$ such that $\phi$ satisfies that $$\eqref{chap03_03_07}$$ and $$\eqref{chap03_03_08}$$.
For all test $\phi^{\prime}: \mathcal{X} \rightarrow [0, 1]$ at level $\alpha$, from $$\eqref{chap03_03_08}$$,


$$
    (\phi - \phi^{\prime})
    (p_{1} - k p_{0})
    \ge
    0
    \quad
    \mu
    \text{-a.e.}
$$

Hence the integral of the equation satisfies

$$
    \int_{\mathcal{X}}
        (\phi - \phi^{\prime})
        (p_{1} - k p_{0})
    \ \mu(x)
    \ge
    0
$$

Form the equation above,

$$
\begin{eqnarray}
    \int_{\mathcal{X}}
        (\phi - \phi^{\prime})
        p_{1}
    \ \mu(x)
    & \ge &
        k
        \int_{\mathcal{X}}
            (\phi - \phi^{\prime})
            p_{0}
        \ \mu(x)
    \nonumber
    \\
    & = &
        k
        \mathrm{E}_{0}
        \left[
            \phi
        \right]
        -
        k
        \mathrm{E}_{0}
        \left[
            \phi^{\prime}
        \right]
    \nonumber
    \\
    & = &
        k
        \left(
            \alpha
            -
            \mathrm{E}_{0}
            \left[
                \phi^{\prime}
            \right]
        \right)
    \ge 0
    \quad
    (\because \phi^{\prime} \text{ is test at level } \alpha)
    \nonumber
\end{eqnarray}
$$

Therefore

$$
    \mathrm{E}_{1}
    \left[
        \phi
    \right]
    \ge
    \mathrm{E}_{1}
    \left[
        \phi^{\prime}
    \right]
    .
$$

**proof of (3)**

Let $\phi^{\prime}$ be most powerful test at level $\alpha$.
As we have already shown in (1), there exist the most powerful test $\phi$ at level $\alpha$.
By definition of $\phi$ and (2), 

$$
    \int_{\mathcal{X}}
        (\phi - \phi^{\prime})
        (p_{1} - k p_{2})
    \ \mu(x)
    \ge
    0
    .
$$

In other hand, $\phi^{\prime}$ is most powerful test at level $\alpha$ so that we have

$$
    \mathrm{E}_{1}
    \left[
        \phi^{\prime}
    \right]
    \ge
    \mathrm{E}_{1}
    \left[
        \phi
    \right]
    .
$$

<div class="QED" style="text-align: right">$\Box$</div>

### Corollary 3.2.1
* $\alpha \in (0, 1)$,
* $\beta \in [0, 1]$
  * powe of the most powerful level $\alpha$ test for hypothesis $$\Theta_{0} := \{0\}$$ and alternatives $$\Theta_{1} := \{1\}$$.

Then

$$
  P_{0} \neq P_{1}
  \Rightarrow
  \alpha < \beta
  .
$$

### proof
Since $\phi \equiv \alpha$ is a level-$\alpha$ test , which has power $\alpha$, $\alpha \le \beta$.
If $\alpha = \beta$, the test $\phi(x) \equiv \alpha$ is most poweful and by Therorem 3.2.1 (iii) must satisfy $$\eqref{chap03_03_08}$$.
Then $p_{0} = p_{1}$ $\mu$-a.e. and henc $P_{0} = P_{1}$.

<div class="QED" style="text-align: right">$\Box$</div>
