---
title: Chapter16-02. Direct Solution of the KKT System
book_title: Numerical Optimization
book_chapter: 16
book_section: 2
---

## 16.2 Direct Solution of the KKT System

#### Theorem 16.3
* $K$
* $A \in \mathbb{R}^{m \times n}$,
    * rank $m$

Then

$$
    \mathrm{inertia}(K)
    =
    \mathrm{inertia}(Z^{\mathrm{T}}GZ)
    +
    (m, m, 0)
    .
$$

If $Z^{\mathrm{T}}GZ$ is positive definite, $\mathrm{inertia}(K) = (n, m, 0)$.

#### proof


<div class="QED" style="text-align: right">$\Box$</div>

$$
\begin{eqnarray}
    x^{*}
    & := &
        Yx_{Y}
        +
        Z x_{Z}
    \nonumber
    \\
    Z
    & \in &
        \mathrm{Null}(A)
    \nonumber
    \\
    Y
    & \in &
        \mathbb{R}^{n - m}
    \nonumber
\end{eqnarray}
$$

By substituting this into the equality constraints,

$$
\begin{eqnarray}
    & &
        Ax = b
    \nonumber
    \\
    & \Leftrightarrow &
        A Y x_{Y}
        +
        A Z x_{Z}
        = b
    \nonumber
    \\
    & \Leftrightarrow &
        A Y x_{Y}
        = b
    .
    \nonumber
\end{eqnarray}
$$

$$
\begin{eqnarray}
    q(x)
    & = &
        \frac{1}{2}
        x^{\mathrm{T}} G x
        +
        c^{\mathrm{T}}
        x
    \nonumber
    \\
    & = &
        \frac{1}{2}
        (Yx_{Y})^{\mathrm{T}} G x
        +
        c^{\mathrm{T}}
        x
\end{eqnarray}
$$

TODO.

<div class="QED" style="text-align: right">$\Box$</div>

### Factoring The Full KKT System



- (1) Since $K$ can be indefinite, we could Gaussian elimination with partial pivoting. This ignores the symmetry.
- (2) Symmetric indefinite factorization in Chapter 3.


For (2), $K$ is decomposed as follows

$$
\begin{eqnarray}
    P^{\mathrm{T}}KP
    =
    LBL^{\mathrm{T}}
    \label{equation_16_12}
\end{eqnarray}
$$

where $P$ is permutation matrix, $L$ is unit lower triangular, and $B$ is block-diagonal with either $1 \times 1$ or $2 \times 2$ blocks.
By substituting the decomposition, we obtain

$$
\begin{eqnarray}
    & &
        K
        \left(
            \begin{array}{c}
                -p
                \\
                \lambda^{*}
            \end{array}
        \right)
        =
        \left(
            \begin{array}{c}
                g
                \\
                h
            \end{array}
        \right)
    \nonumber
    \\
    & \Leftrightarrow &
        PLBL^{\mathrm{T}}P^{\mathrm{T}}
        \left(
            \begin{array}{c}
                -p
                \\
                \lambda^{*}
            \end{array}
        \right)
        =
        \left(
            \begin{array}{c}
                g
                \\
                h
            \end{array}
        \right)
    \nonumber
    \\
    & \Leftrightarrow &
        LBL^{\mathrm{T}}P^{\mathrm{T}}
        \left(
            \begin{array}{c}
                -p
                \\
                \lambda^{*}
            \end{array}
        \right)
        =
        P^{\mathrm{T}}
        \left(
            \begin{array}{c}
                g
                \\
                h
            \end{array}
        \right)
    .
    \nonumber
\end{eqnarray}
$$

To solve the equation,

$$
\begin{eqnarray}
    \text{solve }_{z}
        L z
    & = &
        P^{\mathrm{T}}
        \left(
            \begin{array}{c}
                g
                \\
                h
            \end{array}
        \right)
    \nonumber
    \\
    \text{solve }_{\hat{z}}
        B \hat{z}
    & = &
        z
    \nonumber
    \\
    \text{solve }_{\bar{z}}
        L^{\mathrm{T}} \bar{z}
    & = &
        \hat{z}
    \nonumber
    \\
    \left(
        \begin{array}{c}
            - p
            \\
            \lambda^{*}
        \end{array}
    \right)
    & \leftarrow &
        P \bar{z}
    \nonumber
\end{eqnarray}
$$

### Schur-complement Method
- $G$ is positive definite

From KKT condition, 

$$
\begin{eqnarray}
    -Gp + A^{\mathrm{T}}\lambda^{*}
    & = &
        g
    \nonumber
    \\
    -Ap
    & = &
        h
    .
    \nonumber
\end{eqnarray}
$$

$$
\begin{eqnarray}
    & &
        -Gp + A^{\mathrm{T}}\lambda^{*}
        =
        g
    \nonumber
    \\
    & \Leftrightarrow &
        -Ap
        +
        AG^{-1}A^{\mathrm{T}}\lambda^{*}
        =
        AG^{-1}g
    \nonumber
    \\
    & \Leftrightarrow &
        h
        +
        AG^{-1}A^{\mathrm{T}}\lambda^{*}
        =
        AG^{-1}g
    \nonumber
    \\
    & \Leftrightarrow &
        AG^{-1}A^{\mathrm{T}}\lambda^{*}
        =
        AG^{-1}g
        -
        h
    .
    \label{equation_16_13}
\end{eqnarray}
$$

We can solve the equation with respect to $\lambda^{*}$.

$$
\begin{eqnarray}
    & &
        -Gp
        +
        A^{\mathrm{T}}\lambda^{*}
        =
        g
    \nonumber
    \\
    & \Leftrightarrow &
        Gp
        =
        A^{\mathrm{T}}\lambda^{*}
        -
        g
    .
    \label{equation_16_14}
\end{eqnarray}
$$



$$
\begin{eqnarray}
    \left(
        \begin{array}{cc}
            G & A^{\mathrm{T}}
            \\
            0 & - AG^{-1}A^{\mathrm{T}}
        \end{array}
    \right)
    \label{equation_16_15}
\end{eqnarray}
$$

$AG^{-1}A^{\mathrm{T}}$ is the Schur complenet of $G$ in $K$.


$$
\begin{eqnarray}
    \left(
        \begin{array}{cc}
            G & A^{\mathrm{T}}
            \\
            A & 0
        \end{array}
    \right)^{-1}
    & = &
        \left(
            \begin{array}{cc}
                C & E
                \\
                E^{\mathrm{T}} & F
            \end{array}
        \right)
    \nonumber
    \\
    C
    & := &
        G^{-1} - G^{-1}A^{\mathrm{T}}(AG^{-1}A^{\mathrm{T}})^{-1}AG^{-1}
    \nonumber
    \\
    E
    & := &
        G^{-1}A^{\mathrm{T}}(AG^{-1}A^{\mathrm{T}})^{-1}
    \nonumber
    \\
    F
    & := &
        -(AG^{-1}A^{\mathrm{T}})^{-1}
    .
    \nonumber
\end{eqnarray}
$$


### Null-space method


- Null space method does not require nonsingularity of $G$.


$$
\begin{eqnarray}
    p
    =
    Y p_{Y}
    +
    Z p_{Z}
    \label{equation_16_17}
\end{eqnarray}
$$

where $Z \in \mathbb{R}^{n \times (n - m)}$ null-space matrix, and $Y \in \mathbb{R}^{n \times m}$ such that $[Y \mid Z]$ is nonsingular.
By substituting $p$ into the second equation, we obtain

$$
\begin{eqnarray}
    & &
        -A p
        =
        h
    \nonumber
    \\
    & \Leftrightarrow &
        -A
        \left(
            Y p_{Y}
            +
            Z p_{Z}
        \right)
        =
        h
    \nonumber
    \\
    & \Leftrightarrow &
        -A
        Y p_{Y}
        =
        h
    .
    \label{equation_16_18}
\end{eqnarray}
$$

$$
\begin{eqnarray}
    & &
        -G p
        +
        A^{\mathrm{T}}\lambda^{*}
        =
        g
    \nonumber
    \\
    & \Leftrightarrow &
        - GYp_{Y}
        -
        G Z p_{Z}
        +
        A^{\mathrm{T}}\lambda^{*}
        =
        g
    \nonumber
    \\
    & \Leftrightarrow &
        - Z^{\mathrm{T}}GYp_{Y}
        -
        Z^{\mathrm{T}} G Z p_{Z}
        =
        Z^{\mathrm{T}} g
    \nonumber
    \\
    & \Leftrightarrow &
        Z^{\mathrm{T}}GYp_{Y}
        =
        -
        Z^{\mathrm{T}} g
        -
        Z^{\mathrm{T}} G Z p_{Z}
    .
    \label{equation_16_19}
\end{eqnarray}
$$

Lagrange multiplier is obtaiined by

$$
\begin{eqnarray}
    & &
        -Gp + A^{\mathrm{T}}\lambda^{*}
        =
        g
    & \Leftrightarrow &
        A^{\mathrm{T}}\lambda^{*}
        =
        g
        +
        Gp
    \nonumber
    \\
    & \Leftrightarrow &
        (AY)^{\mathrm{T}}\lambda^{*}
        =
        Y^{\mathrm{T}}
        \left(
            g
            +
            Gp
        \right)
    \label{equation_16_20}
\end{eqnarray}
$$

- Step1. Solve $$\eqref{equation_16_18}$$ with respect to $p_{Y}$.
- Step2. Solve $$\eqref{equation_16_19}$$ with respect to $p_{Z}$.
- Step3. Solve $$\eqref{equation_16_20}$$ with respect to $\lambda^{*}$.




