---
title: Chapter02-02. Centralizers and normalizers, stabilizers and kernels
book_title: Abstract Algebra
book_chapter: 02
book_section: 02
---

## 02-02. Centralizers and normalizers, stabilizers and kernels

### Definition.
* $G$,
    * group
* $A \neq \nonempty$,
    * subset


$$
    C_{G}(A)
    :=
    \{
        g \in G
        \mid
        \forall a \in A,
        \
        gag^{-1}
        =
        a
    \}.
$$

$C_{G}(A)$ is calledthe centralizer of $A$ in $G$.

<div class="end-of-statement" style="text-align: right">■</div>

### Proposition.
* $G$,
* $A \neq \emptyset \subseteq G$,
    * subset

$$
    g a g^{-1}
    =
    a
    \Leftrightarrow
    a g^{-1}
    =
    g^{-1}
    a
    \Leftrightarrow
    ga
    =
    ag
    .
$$

### proof.

<div class="QED" style="text-align: right">$\Box$</div>

### Proposition.
* $G$,
* $A \neq \emptyset \subseteq G$,
    * subset

$C_{A}(G)$ is a subgroup of $G$.

### proof.
$C_{A}(G) \neq \emptyset$ since $1 \in C_{G}(A)$.
Suppose that $a, b \in C_{G}(A)$.

$$
\begin{eqnarray}
    \forall c \in A,
    \
    ab
    c
    (ab)^{-1}
    & = &
        a
        b
        c
        b^{-1}
        a^{-1}
    \nonumber
    \\
    & = &
        a
        c
        a^{-1}
    \nonumber
    \\
    & = &
        c
    \nonumber
\end{eqnarray}
$$

$C_{G}(A)$ is closed under the operation.
Suppose that $a \in C_{G}(A)$.

$$
\begin{eqnarray}
    \forall c \in A,
    \
    a^{-1}
    c
    (a^{-1})^{-1}
    & = &
        a^{-1}
        c
        a
    \nonumber
    \\
    & = &
        a^{-1}
        a
        c
        \quad
        (\because a \in C_{G}(A))
    \nonumber
    \\
    & = &
        c
    .
    \nonumber
\end{eqnarray}
$$

<div class="QED" style="text-align: right">$\Box$</div>

### Definition. center
* $G$,
    * group

$$
    Z(G)
    :=
    \{
        g \in G
        \mid
        \forall g \in G,
        \
        gx
        =
        xg
    \}
$$

$Z(G)$ is called the center of $G$.

<div class="end-of-statement" style="text-align: right">■</div>

### Remark
$$
    C_{G}(G)
    =
    Z(G)
    .
$$

<div class="end-of-statement" style="text-align: right">■</div>

### Definition. normalizer
* $G$,
    * group

$$
\begin{eqnarray}
    gAg^{-1}
    & := &
        \{
            gag^{-1}
            \mid
            a \in A
        \}
    \nonumber
    \\
    N_{G}(A)
    & := &
        \{
            g \in G
            \mid
            gAg^{-1}
            =
            A
        \}
    \nonumber
    \\
\end{eqnarray}
    .
$$

<div class="end-of-statement" style="text-align: right">■</div>

### Remark
$$
    C_{G}(A)
    \subseteq
    N_{G}(A)
    .
$$

$gag^{-1} \in A$ is weaker condition than $gag^{-1} = a$.
$C_{G}(A)$ requires that $gag^{-1}$ exactly is equal to $a$.

<div class="end-of-statement" style="text-align: right">■</div>
