---
title: Chapter07-06. The chinise remainder theorem
book_title: Abstract Algebra
book_chapter: 07
book_section: 06
---

## 07-06. The chinise remainder theorem
Thorughout this section we assume

* All rings are commutative with indentity $1 \neq 0$,


### Definition. comaximal
* $R$,
    * ring
* $A, B \subseteq R$,
    * ideals

$A$ and $B$ are said to be comaximal if $A + B = R$.

<div class="end-of-statement" style="text-align: right">â– </div>

### Proposition.
* $R$,
    * ring
* $A, B \subseteq R$,
    * ideals

The followings are equivalent.

* (i)

$$
    \exists a \in A,
    \
    b \in B,
    \
    \text{ s.t. }
    \
    a + b = 1
    ,
$$

* (ii) $A$ and $B$ are comaximal.

### proof.
(i) $\Rightarrow$ (ii)

Let $c \in R$.
By assumpation,

$$
    ca + cb
    =
    c
    .
$$

Since $A$ and $B$ are ideals, $ca \in A$ and $cb \in B$.

(i) $\Leftarrow$ (ii)
We know $1 \in R$.

<div class="QED" style="text-align: right">$\Box$</div>

### Theorem 17. Chinise Remainder Theorem
* $R$,
* $A_{1}, \ldots, A_{k}$,
    * ideals
* $\phi: R \rightarrow R/A_{1} \times \cdots \times R/A_{k}$,

$$
    \phi(r)
    :=
    (r + A_{1}, \ldots, r + A_{k})
    .
$$

$\phi$ is a ring homomorphisim with kernel $A_{1} \cap A_{2} \cap \cdots \cap A_{k}$.
If $$\forall i, j \in \{1, \ldots, k\}$$ with $i \neq j$ the ideals $A_{i}$ and $A_{j}$ are comaximal, then

* (i) $\phi$ is surjective,
* (ii)

$$
    A_{1} \cap \cdots A_{k}
    =
    A_{1} \cdots A_{k}
    .
$$

That is,

$$
    R/(A_{1}\cdots A_{k})
    \cong
    R/A_{1}
    \times
    R/A_{2}
    \times
    \cdots
    \times
    R/A_{k}
    .
$$

### proof.
We first show that 

$$
    \mathrm{Ker}\phi
    =
    A_{1}
    \cap
    \cdots
    \cap
    A_{k}
    .
$$

It's easy to see $\mathrm{Ker}\phi_{i} = A_{i}$ for all $$i \in \{1, \ldots, k\}$$.
Since $\phi = (\phi_{1}, \ldots, \phi_{k})$, $\mathrm{Ker}\phi = A_{1} \cap \cdots \cap A_{k}$.

Now we show the statement for comaximal part by induction.
In case of $k = 2$.
Let $A = A_{1}$ and $B := A_{2}$.
Suppose that $A + B = R$.

(i) There exists $x \in A$, $y \in B$ such that

$$
    x + y = 1.
$$

This equation show that

$$
\begin{eqnarray}
    \phi(x)
    & = &
        (x + A, x + B)
    & = &
        (0, 1)
    \nonumber
    \\
    \phi(y)
    & = &
        (y + A, y + B)
    & = &
        (1, 0)
    \nonumber
\end{eqnarray}
$$

Then

$$
\begin{eqnarray}
    \forall [r_{1}]_{A} \in R/A,
    \forall [r_{2}]_{B} \in R/B,
    \
    \phi(r_{1}x + r_{2}y)
    & = &
        \phi(r_{1})\phi(x)
        +
        \phi(r_{2})\phi(y)
    \nonumber
    \\
    & = &
        (r_{1} + A, r_{1} + B)
            (0, 1)
        +
        (r_{2} + A, r_{2} + B)
            (1, 0)
    \nonumber
    \\
    & = &
        (0, r_{1} + B)
            (0, 1)
        +
        (r_{2} + A, 0)
            (1, 0)
    \nonumber
    \\
    & = &
        (r_{2} + A, r_{1} + B)
    \nonumber
    \\
    & = &
        ([r_{2}]_{A}, [r_{1}]_{B})
    .
\end{eqnarray}
$$

Thus, $\phi$ is surjective.

(ii)

$A$, $B$ are ideals so that $$\{0\} \in A \cap B \neq \emptyset$$.
It always holds $AB \subseteq A \cap B$ by a porposition in Section 7.3.
Since $A$ and $B$ are comaximal, for any $c \in A\ cap B$,

$$
    c
    =
    c1
    =
    cx + cy
    =
    xc + cy
    \in
    AB
    .
$$

Thus, $A \cap B = AB$.

Suppose that the statement holds up to $k = n-1$.
We show that in case of $k = n$.
Let $A := A_{1}$, $B := A_{2}, \ldots A_{k}$.
We only need to show that $A$ and $B$ are comaximal.
By asusmpation that $A_{1}, \ldots, A_{k}$ are pair-wise comaximal, there are elements $x_{i} \in A_{1}$, $y_{i} \in A_{i}$

$$
    \forall i \in \{2, \ldots, k\},
    \
    x_{i} + y_{i} = 1
    .
$$

Since $$[x_{i}]_{A_{1}}$$, $$x_{i} + y_{i} \equiv y_{i} (\mathrm{mod}\ A_{1})$$.
Hence

$$
    1
    =
    (x_{2} + y_{2})
    (x_{3} + y_{3})
    \cdots
    (x_{k} + y_{k})
$$

By expanding RHS, we see that RHS is an element of $$A_{1} + (A_{2} \cdots A_{k})$$.


<div class="QED" style="text-align: right">$\Box$</div>


## Reference
