---
title: Chapter07-03. Ring homomorphisms and quotient rings
book_title: Abstract Algebra
book_chapter: 07
book_section: 03
---

## 07-03. Ring homomorphisms and quotient rings

### Definiiton. ring homomorphisim
* $R$, $S$,
    * ring
* $\phi: R \rightarrow S$,

$\phi$ is said to be ring homomorphism if

* (i) $\phi(a + b) = \phi(a) + \phi(b)$
* (ii) $\phi(ab) = \phi(a)\phi(b)$

<div class="end-of-statement" style="text-align: right">■</div>

### Definiiton. kernel of ring homomorphisim
* $R$, $S$,
    * ring
* $\phi: R \rightarrow S$,
    * ring homomorphisim

The kernel of the $\phi$, denoted $\mathrm{ker}\phi$, is 

$$
    \mathrm{ker}\phi
    :=
    \{
        x \in R
        \mid
        \phi(x) = 0
    \}
    .
$$

<div class="end-of-statement" style="text-align: right">■</div>

### Definiiton. isomorphisim
* $R$, $S$,
    * ring
* $\phi: R \rightarrow S$,
    * ring homomorphisim


A bijective ring homomorphisim is called an isomorphisim

<div class="end-of-statement" style="text-align: right">■</div>

### Examples

<div class="end-of-statement" style="text-align: right">■</div>

### Proposition 5.
* $R, S$,
    * ring
* $\phi:R \rightarrow S$,
    * homomorphisimo

* (1) $\mathrm{Im}\phi$ is a subring of $S$,
* (2) $\mathrm{ker}\phi$ is a subring of $R$,
    * $\forall a \in R$, $b \in \mathrm{ker}\phi$, $ab \in \mathrm{ker}\phi$,

### proof.
(1)

$s_{1}, s_{2} \in \mathrm{im}\phi$, then $s_{1} := \phi(r_{1}), s_{2} := \phi(s_{2})$ for some $r_{1}, r_{2} \in R$.
Then

$$
\begin{eqnarray}
    \phi(r_{1} - r_{2})
    & = &
        s_{1} - s_{2}
        \in 
    \nonumber
    \\
    \phi(r_{1}r_{2})
    & = &
        s_{1}s_{2}
    \nonumber
\end{eqnarray}
$$

$\mathrm{im}\phi$ is closed under subtraction and multiplication.
Thus, $\mathrm{im}\phi$ is subring.

(2)

If $\alpha, \beta \in \mathrm{ker}\phi$, $\phi(\alpha) = \phi(\beta) = 0$.

$$
\begin{eqnarray}
    \phi(\alpha - \beta)
    & = &
        0
        \in 
    \nonumber
    \\
    \phi(\alpha\beta)
    & = &
        0
    \nonumber
\end{eqnarray}
$$

$\mathrm{ker}\phi$ is closed under subtraction and multiplication.
Thus, $\mathrm{ker}\phi$ is subring.
Similary,

$$
\begin{eqnarray}
    \forall r \in \mathbb{R},
    \
    \phi(r\alpha)
    & = &
        \phi(r)
        0
    \nonumber
    \\
    & = &
        0
    \nonumber
    \\
    \
    \phi(\alpha r)
    & = &
        0
        \phi(r)
    \nonumber
    \\
    & = &
        0
    \nonumber
\end{eqnarray}
$$

<div class="end-of-statement" style="text-align: right">■</div>

### Definition. ideal
* $R$,
    * ring
* $I \subset I$,
* $r \in R$,


(1) $$rI := \{ra \mid a \in I\}$$, $$Ir := \{a r \mid a \in I\}$$,

(2) $I$ is said to be left ideal if

* (i) $I$ is a subring of $R$,
* (ii) $r \in R$, $rI \subseteq I$,

(2) $I$ is said to be right ideal if

* (i)
* (ii) $r \in R$, $Ir \subseteq I$,

(3) $I$ is said to be ideal if $I$ is left and right ideal.

<div class="end-of-statement" style="text-align: right">■</div>

### Definition. arithmetrics of ideals
* $R$,
    * commutative ring
* $I, J \subseteq R$,
    * ideals

* (1) $$I + J := \{a + b \mid a \in I, b \in J\}$$,
* (2) $$IJ := \{ \sum_{i} a_{i}b_{i} \mid k \in \mathbb{N}, a_{i} \in I, b_{i} \in J\}$$,
* (3) For any $n \in \mathbb{N}$, $n$th power of $I$ is defined inductively

$$
    I^{1}
    :=
    I,
    \quad
    I^{n}
    :=
    II^{n-1}.
$$

This is equivalent to 

$$
    I^{n}
    =
    \left\{
        \sum_{i = 1}^{k}
            a_{1}^{i}
            \cdots
            a_{n}^{i}
        \mid
        a_{j}^{i} \in I,
        \
        k \in \mathbb{N},
        \
        j = 1, \ldots, n,
        \
        i = 1, \ldots, k
    \right\}
$$

<div class="end-of-statement" style="text-align: right">■</div>

### Proposition.

* (1) $I + J$ is the smallest ideal containing both $I$ and $J$.
* (2) $IJ$ is a ideal contained in $I \cap J$.

### proof.
(1)

(2)
By definition, $IJ$ is closed under addition.

$$
    \forall r \in R,
    \
    ab \in IJ,
    \
    r(ab)
    =
    (ra)b \in IJ
    .
$$

Thus, $IJ$ is ideal
Let $ab \in IJ$.
Since $J$ is (right) ideal, $a \in R$ and $b \in J$, $ab \in J$.
Similarly, $ab \in I$.
Hence $ab \in I \cap J$.
$I \cap J$ is ideal so that $IJ \subseteq I \cap J$.

<div class="QED" style="text-align: right">$\Box$</div>

## Reference
