---
title: Chapter04-04. Equivalence of Categories
book_title: Categories for the working mathematician
book_chapter: 04
book_section: 04
---

## 04-04. Reflective Subcategories

#### Definition
- $A, C$,
    - category
- $S: A \rightarrow C$,
    - functor

$S$ is said to be an isomorphism of categories if there is a funcotr $T: C \rigtharrow A$ such that

$$
    TS = I: A \rightarrow A
$$

and

$$
    ST = I: C \rightarrow C.
$$

<div class="end-of-statement" style="text-align: right">■</div>

#### Proposition
- $A, C$,
    - category
- $S: A \rightarrow C$
    - functor

The identity natural transformations

$$
    \eta: I \Rightarrow ST
$$

$$
    \epsilon: TS \Rightarrow I.
$$

Then $\langle T, S, \eta, \epsilon \rangle: C \rightarrow A$ is an adjunction.

#### proof

<div class="QED" style="text-align: right">$\Box$</div>


#### Definition
- $S: A \rightarrow C$,
    - functor

$S$ is said to be an equivalence of categories if there is a functor $T: C \rightarrow A$ and natural isomorphisms $\eta: ST \Rightarrow I$ and $\epsilon: TS \Rightarrow I$.

<div class="end-of-statement" style="text-align: right">■</div>


#### Definition
- $C$
    - category
- $A \subseteq C$,
    - subcategory

$A$ is said to be a skelton of $C$ if $A$ is a full subcategory and for any $c \in C$, there is unique $a \in A$ such that $c \cong a$.

<div class="end-of-statement" style="text-align: right">■</div>

#### Example
- $C$
    - category
- $A \subseteq C$,
    - skelton of $C$

$A$ is equivalent to $C$ and the inclusion $K: A \rightarrow C$ is equivalence of $C$.

For any $c$ there is a unique isomorphic object $a \in A$.
Let $T: C \rightarrow A$ be defined as below

$$
    Tc := h_{c}(c)
$$

$$
    f: c \rightarrow c^{\prime},
    \
    (Tf)(a)
    :=
    T(fh_{c}^{-1}(a))
    =
    h_{c^{\prime}}((fh_{c}^{-1}(a)))
$$

where $h_{c}: c \equiv a$ is the isomorphism.

$T$ is a functor.

$$
\begin{eqnarray}
    f: c \rightarrow c^{\prime},
    \
    g: c^{\prime} \rightarrow c^{\prime\prime},
    \
    (Tg) \circ (Tf)(h_{c}^{-1}(a)
    & = &
        (Tg)(T(f(h_{c}^{-1}(a))))
    \nonumber
    \\
    & = &
        (Tg)(h_{c^{\prime}}^{-1}(f(h_{c}^{-1}(a))))
    \nonumber
    \\
    & = &
        T(g(h_{c^{\prime}}^{-1}(h_{c^{\prime}}^{-1}(f(h_{c}^{-1}(a))))))
    \nonumber
    \\
    & = &
        T(g(f(h_{c}^{-1}(a))))
    \nonumber
    \\
    & = &
        T(g \circ f (h_{c}^{-1}(a)))
    \nonumber
    \\
    & = &
    T(g \circ f)(a)
    \nonumber
\end{eqnarray}
$$

We define the natural transofmration $\theta: I \Rightarrow KT$.

$$
    \theta_{c}: Ic \rightarrow KTc,
    \
    \theta_{c}(Ic)
    :=
    h_{c}(c)
    .
$$

$$
\begin{eqnarray}
    f: c \rightarrow c^{\prime},
    \
    (KTf)\theta_{c}(Ic)
    & = &
        (KTf)(h_{c}(c))
    \nonumber
    \\
    & = &
        (KT)(f(c))
    \nonumber
    \\
    & = &
        (KT)(h_{c^{\prime}}h_{c^{\prime}}^{-1}(f(Ic)))
    \nonumber
    \\
    & = &
        (KT)(h_{c^{\prime}}) \circ (KT)(h_{c^{\prime}}^{-1}(f(Ic)))
    \nonumber
    \\
    & = &
        (KT)(h_{c^{\prime}}) \circ (KT)(f(Ic))
\end{eqnarray}
$$

<div class="end-of-statement" style="text-align: right">■</div>


