---
title: Chapter01-04. Natural Transformations
book_title: Categories for the working mathematician
book_chapter: 01
book_section: 04
---

## 01-04. Natural Transformations

#### Definition natural transformations
- $S, T: C \rightarrow B$,
    - functors
- $\tau: S \dot{\rightarrow} T$,
    $\tau_{c} := \tau c: Sc \rightarrow Tc$

$\tau$ is said to be natural transformation if the diagram is 

$$
\begin{CD}
    c \in C
    \\
    @V{f}VV
    \\
    c^{\prime} \in C
\end{CD}
\quad
\begin{CD}
    Sc @>{\tau c}>> Tc
    \\
    @V{Sf}VV    @V{Tf}VV
    \\
    Sc^{\prime} @>{\tau c^{\prime}}>>  Tc^{\prime}
\end{CD}
$$

commutative.

When this holds, $\tau_{c}: Sc \rightarrow Tc$ is said to be natural in $c$.

<div class="end-of-statement" style="text-align: right">■</div>


#### Definition natural isomorphism
- $S, T: C \rightarrow B$,
    - functors
- $\tau: S \dot{\rightarrow} T$,
    - $\tau_{c} := \tau c: Sc \rightarrow Tc$
    - natural transformation

$\tau$ is said to be natural isomorhism if for all $c \in C$, $\tau_{c}$ is isomorphism.

<div class="end-of-statement" style="text-align: right">■</div>


#### Example1


<div class="end-of-statement" style="text-align: right">■</div>


#### Example2
- $G$,
    - group

$$
    g, h \in G,
    \quad
    [g, h]
    :=
    g^{-1}h^{-1}gh.
$$

is called a commutator of $G$.

$$
    [G, G]
    :=
    \{
        [g_{1}, h_{1}] \cdot [g_{n}, h_{n}] 
        \mid
        g_{k}, h_{k} \in G,
        \
        n \in \mathbb{N}
    \}
    .
$$

$[G, G]$ is a normal subgroup of $G$.
Since $e = [e, e]$, $[e, e] \in [G, G]$.

$$
    [e, e] = e
    .
$$

Since

$$
\begin{eqnarray}
    [g, h]
    [h, g]
    & = &
        g^{-1} h^{-1}
        gh
        h^{-1} g^{-1}
        hg
    \nonumber
    \\
    & = &
        e,
    \nonumber
\end{eqnarray}
$$

$$
\begin{eqnarray}
    \left(
        [g_{1}, h_{1}]
        \cdots
        [g_{n}, h_{n}]
    \right)^{-1}
    & = &
        [h_{n}, g_{n}]
        \cdots
        [h_{1}, g_{1}]
        \in
        [G, G]
    .
    \nonumber
\end{eqnarray}
$$

Moreover, since for all $g \in G$,

$$
\begin{eqnarray}
    ([g_{1}, h_{1}])^{g}
    & = &
        g
        g_{1}^{-1}h_{1}^{-1}g_{1}h_{1}
        g^{-1}
    \nonumber
    \\
    & = &
        (g g_{1}^{-1} g^{-1})
        (gh_{1}^{-1}g^{-1})
        (gg_{1} g^{-1})
        (gh_{1} g^{-1})
    \nonumber
    \\
    & = &
        (g_{1}^{g})^{-1}
        (h_{1}^{g})^{-1}
        (g_{1}^{g})
        (h_{1}^{g})
    \nonumber
    \\
    & = &
        [g_{1}^{g}, h_{1}^{g}],
    \nonumber
\end{eqnarray}
$$

$[g_{1}^{g}, g_{1}^{g}] \in [G, G]$.
Thus, $[G, G]$ is a normal subgroup.

$$
    G^{*}
    :=
    G / [G, G]
    .
$$

$$
\begin{eqnarray}
    p_{G}: G \rightarrow G^{*}
    \nonumber
    \\
    p_{G}(g)
    & := &
        [g]
    \nonumber
    .
\end{eqnarray}
$$



<div class="end-of-statement" style="text-align: right">■</div>
