---
title: Chapter04-01. Adjoints
book_title: Categories for the working mathematician
book_chapter: 04
book_section: 01
---

## 04-01. Adjunctions

#### Definition Adjunction
- $A, X$,
    - category
- $F: X \rightarrow A$,
    - functor
- $G: A \rightarrow F$,
    - functor
- $$\mathcal{S} = \{f: A(Fx, a) \rightarrow X(x, Ga) \mid x \in X, a \in A\}$$,
- $\phi: X \times A \rightarrow \mathcal{S}$,

A triple $\langle F, G, \phi \rangle$ is said to be an adjunction from $X$ to $A$ if for all $x \in X$, $a \in A$, $\phi_{x, a}$ is a bijection

$$
\begin{equation}
    \phi_{x,a}: A(Fx, a) \simeq X(x, Ga)
    \label{chap04_01_eq_definition_adjunction}
\end{equation}
$$

and natural in $x$ and $a$.
That is, the diagrams are commute.

$$
\begin{CD}
    a \\
    @V{k}VV \\
    a^{\prime}
\end{CD}
\qquad
\begin{CD}
    A(Fx, a) @>{\phi_{x, a}}>> X(x, Ga)
    \\
    @V{k_{*}}VV    @V{(Gk)_{*}}VV
    \\
    A(Fx, a^{\prime}) @>{\phi_{x, a^{\prime}}}>> X(x, Ga^{\prime})
\end{CD}

\qquad
\qquad
\qquad

\begin{CD}
    x \\
    @V{k}VV \\
    x^{\prime}
\end{CD}
\qquad
\begin{CD}
    A(Fx, a) @>{\phi_{x, a}}>> X(x, Ga)
    \\
    @V{k_{*}}VV    @V{(Gk)_{*}}VV
    \\
    A(Fx^{\prime}, a) @>{\phi_{x^{\prime}, a}}>> X(x^{\prime}, Ga)
\end{CD}
$$

For all $a$, the naturality holds for the two functors $A(-, a) \circ F: X \rightarrow \mathrm{Set}$ and $X(-, Ga): X \rightarrow \mathrm{Set}$.

For all $x$, the naturality holds for the two functors $A(Fx, -): A \rightarrow \mathrm{Set}$ and $X(x, -) \circ G: A \rightarrow \mathrm{Set}$.

<div class="end-of-statement" style="text-align: right">■</div>

#### Definition
- $k: a \rightarrow a^{\prime}$,
- $h: x^{\prime} \rightarrow x$,

$$
    k_{*} := A(Fx, k),
    \
    h^{*} := X(h, Ga)
    .
$$

- $Gk: Ga \rightarrow Ga^{\prime}$,
- $Fh: Fx^{\prime} \rightarrow Fx$,

$$
    (Fh)_{*}
    :=
    A(Fx, Fh),
    \
    (Gk)^{*}
    :=
    X(Gk, Ga).
$$

<div class="end-of-statement" style="text-align: right">■</div>

#### Example
- $K$,
    - field
- $A := \mathrm{Vct}_{K}$,
- $X := \mathrm{Set}$,
- $F: X \rightarrow A$,
    - functor
    - object function: $G(x) = v_{x}$ is a vector space with basis $x$, 
    - arrow function: $g: x \rightarrow y$, $F(g): v_{x} \rightarrow v_{y}$
- $G := U: A \rightarrow X$,
    - forgetful functor

Any $g: x \rightarrow U(v_{y})$ can be extended to the unique linear function

$$
    f(\sum_{i} r_{i} x_{i}) := \sum_{i}r_{i}g(x_{i}).
$$

The restriciton of $f$ to $x$ is the inverse of the mapping.
So the mapping 

$$
    \phi_{x, w}: A(Fx, w) \rightarrow X(x, U(w))
$$

is a bijection.
The arrow function of $F$ is

$$
    g: x \rightarrow y,
    \quad
    F(g) = \phi_{x, F(y)}^{-1}
    .
$$

$\phi$ is natural in $x$ and $w$.

For all $w$, the naturality holds for the two functors $A(-, w) \circ F: X \rightarrow \mathrm{Set}$ and $X(-, U(w)): X \rightarrow \mathrm{Set}$.

$$
\begin{CD}
    x^{\prime}
    \\
    @V{h}VV
    \\
    x
\end{CD}
\qquad
\qquad
\qquad
\begin{CD}
    A(Fx, w) @>{\phi_{x, w}}>> X(x, U(w))
    \\
    @V{(A(-, w)\circ F)h}VV    @V{X(-, U(w))h}VV
    \\
    A(Fx^{\prime}, w) @>{\phi_{x^{\prime, w}}}>> X(x^{\prime}, U(w))
\end{CD}
$$

Indeed,

$$
\begin{eqnarray}
    f: Fx \rightarrow w,
    \
    (X(h, U(w)) \circ \phi_{x, w})(f)
    & = &
        X(h, w)\left. f\right|_{x}
    \nonumber
    \\
    & = &
        \left. f\right|_{x} \circ h
    \nonumber
\end{eqnarray}
$$

and

$$
\begin{eqnarray}
    f: Fx \rightarrow w,
    \
    (\phi_{x^{\prime}, w} \circ (A(Fh, w)))(f)
    & = &
        \phi_{x^{\prime}, w} (f \circ Fh)
    \nonumber
    \\
    & = &
        \left. (f \circ Fh) \right|_{x^{\prime}}
    \nonumber
\end{eqnarray}
$$

For all $x$, the naturality holds for the two functors $A(Fx, -): A \rightarrow \mathrm{Set}$ and $X(x, -) \circ U: A \rightarrow \mathrm{Set}$.

$$
\begin{CD}
    w
    \\
    @V{k}VV
    \\
    w^{\prime}
\end{CD}
\qquad
\qquad
\qquad
\begin{CD}
    A(Fx, w) @>{\phi_{x, w}}>> X(x, U(w))
    \\
    @V{A(Fx, -)k}VV    @V{(X(x, -) \circ U)k}VV
    \\
    A(Fx, w^{\prime}) @>{\phi_{x, w^{\prime}}}>> X(x, U(w^{\prime}))
\end{CD}
$$

Indeed,

$$
\begin{eqnarray}
    f: Fx \rightarrow w,
    \
    (((X(x, -) \circ U)k) \circ \phi_{x, w})(f)
    & = &
        X(x, U(k))\left. f\right|_{x}
    \nonumber
    \\
    & = &
        U(k) \circ \left. f\right|_{x}
    \nonumber
\end{eqnarray}
$$

and

$$
\begin{eqnarray}
    f: Fx \rightarrow w,
    \
    (\phi_{x, w^{\prime}} \circ A(Fx, k))(f)
    & = &
        \phi_{x, w^{\prime}} (k \circ f)
    \nonumber
    \\
    & = &
        \left. (k \circ f) \right|_{x}
    .
    \nonumber
\end{eqnarray}
$$

<div class="end-of-statement" style="text-align: right">■</div>


#### Example Free category


<div class="end-of-statement" style="text-align: right">■</div>


#### Definition adjunct
- $f \in A(Fx, a)$,
- $\phi: A(Fx, a) \rightarrow X(x, Ga)$
    - bijection

$\phi$ is said to be the right adjunct of $f$ if $\phi(f) \in X(x, Ga)$.

<div class="end-of-statement" style="text-align: right">■</div>

#### Remark
The right adjunction is natural if

$$
\begin{eqnarray}
    f \in A(Fx, a),
    \
    h: x^{\prime} \rightarrow x,
    \
    k: a \rightarrow a^{\prime},
    \quad
    \phi(k \circ f)
    =
    Gk \circ \phi(f),
    \quad
    \phi(f \circ Fh)
    =
    \phi(f) \circ h.
    \label{chap04_01_eq_right_adjunct}
\end{eqnarray}
$$

The above is equivalent to 

$$
\begin{eqnarray}
    g \in A(x, Ga),
    \
    h: x^{\prime} \rightarrow x,
    \
    k: a \rightarrow a^{\prime},
    \quad
    \phi^{-1}(g \circ h)
    =
    \phi^{-1}g \circ Fh
    \quad
    \phi^{-1}(Gk \circ g)
    =
    k \circ \phi^{-1}(g)
    .
    \label{chap04_01_eq_left_adjunct}
\end{eqnarray}
$$

<div class="end-of-statement" style="text-align: right">■</div>

#### Definition adjoint
- $\langle F, G, h \rangle$,
    - adjunciton

$F$ is called left-adjoint for $G$.
$G$ is called right-adjoint for $F$.

<div class="end-of-statement" style="text-align: right">■</div>


#### Theorem 1
- $\langle F, G, \phi \rangle: X \rightarrow A$,
    - adjunction

(1) A natural transformation $\eta: I_{X} \Rightarrow GF$ such that for all $x \in X$ the arrow $\eta_{x}$ is universal to $G$ from $x$, and the right adjunct of each $f: Fx \rightarrow a$ is 

$$
\begin{equation}
    \phi(f)
    =
    Gf \circ \eta_{x}: x \rightarrow Ga
    \label{chap04_01_theorem_01_eq_01}
\end{equation}
$$

(2) A natural transformation $\epsilon: FG \Rightarrow I_{A}$ such that for all $a \in A$ the arrow $\epsilon_{a}$ is universal to $a$ from $F$, and left ajunct of the $g: x \rightarrow Ga$ is

$$
\begin{equation}
    \phi^{-1}g
    =
    \epsilon_{a} \circ Fg: Fx \rightarrow a.
    \label{chap04_01_theorem_01_eq_02}
\end{equation}
$$


Moreover, the following compostes are the indentites.

$$
\begin{equation}
    G \xrightarrow{\eta G} GFG \xrightarrow{G\epsilon} G,
    \quad
    F \xrightarrow{\eta G} FGF \xrightarrow{G\epsilon} F.
    \label{chap04_01_theorem_01_eq_03}
\end{equation}
$$

#### proof
(1)

Let $a := Fx$ in $$\eqref{chap04_01_eq_definition_adjunction}$$.
The bijection

$$
    \phi: A(Fx, Fx) \cong X(x, GFx)
$$

is natural in $Fx$.

By the <a href="{{ site.baseurl }}/book/categories_for_the_working_mathematician/chap03_02.html#proposition-1">proposition 1</a> in Chapter3.2,
there is a universal arrow $\eta_{x}: x \rightarrow GF x := \phi(1_{Fx})$ from $x$ to $G$ taking $S := G: A \rightarrow X$, $r := Fx$, $d := Fx$, $c := x$.
$$\eta_{x}$$ is natural in $Fx$.
Moreover, $$\eta: I_{X} \Rightarrow GF$$ is a natural transformation.
That is, the following diagram commute.

$$
\begin{CD}
    x^{\prime} \\
    @V{h}VV \\
    x
\end{CD}
\qquad
\begin{CD}
    I_{X}x^{\prime} @>{\eta_{x^{\prime}}}>> GF x^{\prime}
    \\
    @V{I_{X}h}VV    @V{GF h}VV
    \\
    I_{X}x @>{\eta_{x}}>> GF x
\end{CD}
$$

Taking $k := Fh: Fx^{\prime} \rightarrow Fx$, 

$$
\begin{eqnarray}
    GFh \circ \eta_{x^{\prime}}
    & = &
        GF h \circ \phi(1_{Fx^{\prime}})
    \nonumber
    \\
    & = &
        Gk \circ \phi(1_{Fx^{\prime}})
    \nonumber
    \\
    & = &
        \phi(k \circ 1_{Fx^{\prime}})
        \quad
        (\because \eqref{chap04_01_eq_right_adjunct})
    \nonumber
    \\
    & = &
        \phi(1_{Fx^{\prime}} \circ k)
    \nonumber
    \\
    & = &
        \phi(1_{Fx^{\prime}} \circ Fh)
    \nonumber
    \\
    & = &
        \phi(1_{Fx^{\prime}}) \circ h
        \quad
        (\because \eqref{chap04_01_eq_right_adjunct})
    \nonumber
\end{eqnarray}
$$

$$
\begin{CD}
    A(Fx^{\prime}, Fx^{\prime})
        @>{(Fh)_{*}}>>
        A(Fx^{\prime}, Fx)
        @<{(Fh)^{*}}<<
        A(Fx, Fx)
    \\
    @V{\phi}VV    @V{\phi}VV  @V{\phi}VV
    \\
    X(x^{\prime}, GFx^{\prime})
        @>{(GFh)_{*}}>>
        X(x^{\prime}, GFx)
        @<{h^{*}}<<
        X(x, GFx)
\end{CD}
$$

where $$h^{*} := X(h, 1_{GFx})$$ and $$h_{*} := X(1_{x^{\prime}}, h)$$, $h:x^{\prime} \rightarrow x$.


$$
\begin{eqnarray}
    f: Fx \rightarrow a,
    \
    \phi(f)
    & = &
        G(f) \eta_{x}
\end{eqnarray}
$$

Indeed,

$$
\begin{eqnarray}
    \phi(f)
    & = &
        \phi(f \circ 1_{Fx})
    \nonumber
    \\
    & = &
        G(f) \circ \phi(1_{Fx})
        \quad
        (\because \eqref{chap04_01_eq_left_adjunct})
    \nonumber
    \\
    & = &
        G(f) \circ \eta_{x}
    \nonumber
\end{eqnarray}
$$

$$
\begin{CD}
    A(Fx, Fx) @>{\phi_{x, Fx}}>> X(x, GFx)
    \\
    @V{f_{*}}VV    @V{(Gf)_{*}}VV
    \\
    A(Fx, a) @>{\phi_{x, a}}>> X(x, Ga)
\end{CD}
$$

<div class="QED" style="text-align: right">$\Box$</div>

#### Definition unit, counit
- $\langle F, G, \phi \rangle$
    - adjunction
- $\eta: I_{X} \Rightarrow GF$
    - natural transformation in the theorem
- $\epsilon: FG \Rightarrow I_{A}$
    - natural transformation in the theorem

$\eta$ is called the unit of the adjunction. $\epsilon$ is called the counit of the adjunction.

<div class="end-of-statement" style="text-align: right">■</div>

#### Example
In the example of vector spaces,

$$
    \eta_{x} := \phi_{x, Fx}(1_{x}): Fx \rightarrow Fx.
$$

is a mapping from indentity map on a set $x$ to identity of a vector space $Fx$.

$$
    \epsilon_{w} := \phi_{Uw, w}(1_{w}): Uw \rightarrow Uw
$$

is a mapping from an isomorphism on a vector space $w$ to indentity map of a set $Uw$.

<div class="end-of-statement" style="text-align: right">■</div>

#### Theorem 2
- $\langle F, G, \phi \rangle: X \rightarrow A$,
    - adjunction

Each ajunction is completely determiend by one of the items below.

(i)

- $F: X \rightarrow A$,
- $G: A \rightarrow X$,
- $\eta: 1_{X} \Rightarrow GF$,
    - natural transformation
    - $\eta_{x}: x \rightarrow GFx$ is universal to $G$ from $x$

Then $\phi$ is defined by $$\eqref{chap04_01_theorem_01_eq_01}$$.

(ii)

- $G: A \rightarrow X$,
- $\eta: 1_{X} \Rightarrow GF$,
    - natural transformation
    - $\eta_{x}: x \rightarrow GFx$ is universal to $G$ from $x$


(iii)

- $F: X \rightarrow A$, $G: A \rightarrow X$,
    - functors
- $\epsilon: FG \Rightarrow I_{A}$
    - natural transformation
    - $\epsilon_{a}: FGa \rightarrow a$ is universal from $F$ to $a$.

$\phi^{-1}$ is defined in $$\eqref{chap04_01_theorem_01_eq_02}$$.


(iv)

- $F: X \rightarrow A$,
    - functors

For each $a \in A$, $G_{0}a \in X$, $\epsilon_{a}: FG_{0} \rightarrow a$ is universal from $F$ to $a$.

(v)

- $F: X \rightarrow A$, $G: A \rightarrow X$,
    - functors
- $\eta: I_{X} \Rightarrow GF$, $\epsilon: FG \Rightarrow I_{A}$,
    - natural transformations
    - satisfies $$\eqref{chap04_01_theorem_01_eq_03}$$,

$\phi$ is defined by $$\eqref{chap04_01_theorem_01_eq_01}$$ and $\phi^{-1}$ is defined by  $$\eqref{chap04_01_theorem_01_eq_01}$$.

#### proof




<div class="QED" style="text-align: right">$\Box$</div>
