---
title: Chapter5. The Central Limit Theorem
book_title: Probability and Measure
book_chapter: 5
book_section: 27
---
## 5-27 The Central Limit Theorem
In this section,

* $N$,
    * a r.v. with standard normal distribution

$$
    P(N \in A)
    =
    \frac{
        1
    }{
        \sqrt{2 \pi}
    }
    \int_{A}
        e^{- x^{2}/2}
    \ dx
    .
$$

#### Theorem 27.1
* $c \in \mathbb{R}^{n}$,
* $\sigma > 0$,
* $$\{X_{n}\}_{n \in \mathbb{N}}$$,
    * independent sequence of r.v.s with mean $c$ and $\sigma^{2}$

If

$$
    S_{n}
    :=
    \sum_{i=1}^{n}
        X_{i}
    ,
$$

$$
    \frac{
        S_{n} - nc
    }{
        \sigma \sqrt{n}
    }
    \overset{d}{\rightarrow}
    N
    ,
$$

$\mu$ is said to be complete if

$$
    N \in \mathcal{A},
    \
    \mi(N) = 0,
    \
    \Rightarrow
    \
    \forall S \subseteq N,
    \
    S \in \mathcal{A}
$$

<div class="end-of-statement" style="text-align: right">â– </div>


#### Lemma 1
* $z_{1}, \ldots, z_{m}$,
    * complex numbers of moduls at most 1
* $w_{1}, \ldots, z_{m}$,
    * complex numbers of moduls at most 1

$$
    \abs{
        z_{1} \cdots z_{m}
        -
        w_{1} \cdots w_{m}
    }
    \le
    \sum_{k=1}^{m}
        \abs{
            z_{k} - w_{k}
        }
    .
$$

#### proof
Let $m = 2$.

$$
\begin{eqnarray}
    (z_{1} - w_{1})
    z_{2}
    +
    w_{1}
    (z_{2} - w_{2})
    & = &
        z_{1}z_{2} - w_{1}z_{2}
        +
        w_{1}z_{2} - z_{1}z_{2}
    \nonumber
    \\
    & = &
        z_{1}z_{2}
        - w_{1}w_{2}
    \nonumber
\end{eqnarray}
$$

Thus,

$$
\begin{eqnarray}
    \abs{
        z_{1}z_{2}
        - w_{1}w_{2}
    }
    & \le &
        \abs{
            (z_{1} - w_{1})
            z_{2}
        }
        +
        \abs{
            w_{1}
            (z_{2} - w_{2})
        }
    \nonumber
    \\
    & \le &
        \abs{
            (z_{1} - w_{1})
        }
        +
        \abs{
            (z_{2} - w_{2})
        }
    .
    \nonumber
\end{eqnarray}
$$

Suppose that the statement holds up to $m = n - 1$.
Then we prove the statement in case of $m = n$.

$$
\begin{eqnarray}
    (z_{1} - w_{1})
    z_{2}\cdots z_{m}
    +
    w_{1}
    (z_{2} \cdots z_{m} - w_{2} \cdots w_{m})
    & = &
        z_{1}\cdots z_{m}
        -
        w_{1}z_{2} \cdots z_{m}
        +
        w_{1}z_{2} \cdots z_{M}
        -
        w_{1}w_{2} \cdots w_{m}
    \nonumber
    \\
    & = &
        z_{1} \cdots z_{m}
        -
        w_{1} \cdots w_{m}
    \nonumber
\end{eqnarray}
$$

Thus,

$$
\begin{eqnarray}
    \abs{
        z_{1} \cdots z_{m}
        -
        w_{1} \cdots w_{m}
    }
    & \le &
        \abs{
            (z_{1} - w_{1})
            z_{2}\cdots z_{m}
        }
        +
        \abs{
            w_{1}
            (z_{2} \cdots z_{m} - w_{2} \cdots w_{m})
        }
    \nonumber
    \\
    & \le &
        \abs{
            (z_{1} - w_{1})
        }
        +
        \abs{
            (z_{2} \cdots z_{m} - w_{2} \cdots w_{m})
        }
    \nonumber
    \\
    & \le &
        \abs{
            (z_{1} - w_{1})
        }
        +
        \sum_{i=2}^{m}
            \abs{
                (z_{i} - w_{i})
            }
    .
    \nonumber
\end{eqnarray}
$$

<div class="QED" style="text-align: right">$\Box$</div>


