---
title: On the electrodynamics of moving bodies
---

## On the electrodynamics of moving bodies


### 3. Theory of the Transformation of Co-ordinates and Times from a Stationary Sytem to another System in Uniform Motion of Translation Relatively to the Former

* $(x, y, z)$, $t$,
    * stationary system
* $(\xi , \eta, \zeta)$, $\tau$,
    * moving system


Assumptions

(1)

There exists $f$ such that

$$
    \tau
    =
    f(x, y, z, t)
$$


(2)

$f$ is linear


$$
    \tau
    =

$$


(3)

$$
    x^{\prime}
    :=
    x - vt
    .
$$


$$
    \tau_{1} - \tau_{0}
    :=
    \tau_{2} - \tau_{1}
    .
$$

$$
    \tau
    =
    a
    \left(
        t
        -
        \frac{
            v
        }{
            c^{2} - v^{2}
        }x^{\prime}
    \right)
$$

where $a$ is a function $\phi(v)$.
For brevity, we assume that $\tau = 0$ at $(0, 0, 0)$ in $k$, when $t = 0$.

For a ray of light emitted from the origin of the moving sytem $k$ at the time $\tau = 0$ in the direction of the increasing $\xi$,

$$
\begin{eqnarray}
    \xi
    & = &
        c \tau
    \nonumber
    \\
    & = &
        ac
        \left(
            t
            -
            \frac{
                v
            }{
                c^{2} - v^{2}
            }x^{\prime}
        \right)
    .
    \nonumber
\end{eqnarray}
$$

When it is measured in the stationary system,

$$
    \frac{
        x^{\prime}
    }{
        c - v
    }
    =
    t.
$$

If we insert the value of $t$,

$$
\begin{eqnarray}
    \xi
    & = &
        ac
        \left(
            t
            -
            \frac{
                v
            }{
                c^{2} - v^{2}
            }x^{\prime}
        \right)
    \nonumber 
    \\
    & = &
        ac
        \left(
            \frac{
                x^{\prime}
            }{
                c - v
            }x^{\prime}
            -
            \frac{
                v
            }{
                c^{2} - v^{2}
            }x^{\prime}
        \right)
    \nonumber 
    \\
    & = &
        ac
        \left(
            \frac{
                1
            }{
                c - v
            }
            -
            \frac{
                v
            }{
                c^{2} - v^{2}
            }
        \right)
        x^{\prime}
    \nonumber 
    \\
    & = &
        ac
        \left(
            \frac{
                c
            }{
                c^{2} - v^{2}
            }
        \right)
        x^{\prime}
    .
    \nonumber
\end{eqnarray}
$$

In an analogous manner by considering rays moing along the two other axes,
when

$$
    \frac{
        y
    }{
        \sqrt{
            c^{2} - v^{2}
        }
    }
    =
    t,
    \
    x^{\prime}
    =
    0,
$$

then

$$
\begin{eqnarray}
    \eta
    & = &
        c \tau
    \nonumber
    \\
    & = &
        ac
        \left(
            t -
            \frac{
                v
            }{
                c^{2} - v^{2}
            }
            x^{\prime}
        \right)
    \nonumber
\end{eqnarray}
$$

Hence,

$$
\begin{eqnarray}
    \eta
    & = &
        ac t
    \nonumber
    \\
    & = &
        ac
        \frac{
            y
        }{
            \sqrt{
                c^{2} - v^{2}
            }
        }
    .
\end{eqnarray}
$$

Similary,

$$
\begin{eqnarray}
    \zeta
    & = &
        ac
        \frac{
            z
        }{
            \sqrt{
                c^{2} - v^{2}
            }
        }
    .
\end{eqnarray}
$$

Substituting for $x^{\prime} = x - vt$,

$$
\begin{eqnarray}
    \beta
    & := &
        \frac{
            1
        }{
            \sqrt{
                1 - v^{2} / c^{2}
            }
        }
    \nonumber
    \\
    & = &
        \frac{
            c
        }{
            \sqrt{
                c^{2} - v^{2}
            }
        }
    \nonumber
    \\
    \phi(v)
    & := &
        a \beta,
    \nonumber
\end{eqnarray}
$$

$$
\begin{eqnarray}
    \tau
    & = &
        a
        \left(
            t
            -
            \frac{
                v
            }{
                c^{2} - v^{2}
            }
            x^{\prime}
        \right)
    \nonumber
    \\
    & = &
        a
        \left(
            t
            -
            \frac{
                v
            }{
                c^{2} - v^{2}
            }
            (x - vt)
        \right)
    \nonumber
    \\
    & = &
        a
        \left(
            t
            +
            \frac{
                v^{2}
            }{
                c^{2} - v^{2}
            }
            t
            -
            \frac{
                v
            }{
                c^{2} - v^{2}
            }
            x
        \right)
    \nonumber
    \\
    & = &
        a
        \left(
            \beta^{2}t
            -
            \frac{
                v
            }{
                c^{2} - v^{2}
            }
            x
        \right)
    \nonumber
    \\
    & = &
        a
        \left(
            \beta^{2}t
            -
            v \beta^{2}
            \frac{1}{c^{2}}
            x
        \right)
    \nonumber
    \\
    & = &
        \phi(v)
        \beta
        \left(
            t
            -
            \frac{v}{c^{2}}
            x
        \right)
    \nonumber
    .
\end{eqnarray}
$$

$$
\begin{eqnarray}
    \xi
    & = &
        a
        \frac{
            c^{2}
        }{
            c^{2} - v^{2}
        }
        x^{\prime}
    \nonumber
    \\
    & = &
        a
        \beta^{2}
        (x - vt)
    \nonumber
    \\
    & = &
        \phi(v)
        \beta
        (x - vt)
    .
    \nonumber
\end{eqnarray}
$$

$$
\begin{eqnarray}
    \eta
    & = &
        \frac{
            a c
        }{
            \sqrt{c^{2} - v^{2}}
        }y
    \nonumber
    \\
    & = &
        a \beta y
    \nonumber
    \\
    & = &
        \phi(v) y
    .
    \nonumber
\end{eqnarray}
$$

$$
\begin{eqnarray}
    \zeta
    & = &
        \phi(v) z
    .
    \nonumber
\end{eqnarray}
$$

- a spherical wave

At the time $t = \tau = 0$,

Let a spherical wave be emitted at $t = \tau = 0$ with the velocity $c$ in system $K$.
$(x, y, z)$ is a point attained by this wave.

$$
\begin{eqnarray}
        \sqrt{x^{2} + y^{2} + z^{2}}
        =
        ct
        \nonumber
    & \Leftrightarrow &
        x^{2} + y^{2} + z^{2} 
        =
        c^{2} t^{2}
        \nonumber
        .
\end{eqnarray}
$$

## Reference
